lakefile.lean
@@ -9,7 +9,6 @@ lean_lib Paco
 
 lean_lib Tests
 
-lean_lib Standalone
 
 require mathlib from git
   "https://github.com/leanprover-community/mathlib4.git"@"v4.26.0"
